src/tls/KeySchedule.fst
@@ -21,42 +21,227 @@ open HandshakeMessages
 open StatefulLHAE
 open HSCrypto
 
-// KEF.fst/TLSPRF.fst for TLS 1.2
-// CoreCrypto.hkdf for TLS 1.3
+module MM = MonotoneMap
+module MR = FStar.Monotonic.RRef
+module HH = FStar.HyperHeap
 
-// does NOT subsumes the idealized module PRF.fst
-// (we do not solve the circular dependency properly)
+// *** PSK ***
 
+// The constraints for PSK indexes are:
+//  - must be public (as psk index appears in hsId, msId and derived keys)
+//  - must support application-provided PSK as well as RMS-based PSK
+//  - must support dynamic compromise; we want to prove KI of 1RT keys in PSK_DHE
+//    even for leaked PSK (but not PSK-based auth obivously)
+// Implementation style:
+//  - pskid is the TLS PSK identifier, an internal index to the PSK table
+//  - for tickets, the encrypted serialized state is the PSK identifier
+//  - we store in the table the PSK context and compromise status
+let pskid = b:bytes{length b < 65536}
 
-// LONG TERM GLOBAL SECRETS
-// ******************************************
+// TODO: add certificates and other authPSK info
+let psk_context = {
+  allow_early_data: bool;      // New draft 13 flag
+  allow_dhe_resumption: bool;  // New draft 13 flag
+  allow_psk_resumption: bool;  // New draft 13 flag
+  time_created: int;
+  early_ae: aeadAlg;
+  early_hash: hashAlg;
+  resumption_context: option b:bytes{length b <= 64}; // None for application PSK
+}
 
-// For now, we stick to the style of miTLS 0.9
-// to avoid a circular dependency between KEF and StatefulLHAE
+// We rule out all PSK that do not have at least one non-null byte
+// thus avoiding possible confusion with non-PSK for all possible hash algs
+type psk = b:bytes{exists i.{:pattern index b i} index b i <> 0z}
 
+// TODO store the leaked ref in a better region?
+abstract let psk (i:pskid) =
+  psk * ctx:psk_context * leaked:(rref tls_tables_region bool)
+
+// injectivity predicate on map from PSK identities to secret key
+let psk_injective (m:MM.map' pskid psk) =
+  forall i1 i2.{:pattern (MM.sel m i1); (MM.sel m i2)}
+       equalBytes i1 i2 <==> (match MM.sel m i1, MM.sel m i2 with
+                  | Some (psk1,_,_), Some (psk2,_,_) -> equalBytes psk1 psk2
+                  | _ -> True)
+
+// Monotonic table mapping injectively PSK identities to keys and context
+let psk_table : MM.t tls_tables_region pskid psk psk_injective =
+  MM.alloc #TLSConstants.tls_tables_region #pskid #psk #psk_injective
+
+let registered_psk (i:pskid) = is_Some (MM.sel psk_table i)
+
+let get_psk_context (i:pskid{registered_psk i}) =
+  let (_, c, _) = Some.v (MM.sel psk_table i) in c
+
+let leaked_psk (i:pskid{registered_psk i}) =
+  let (_, _, l) = Some.v (MM.sel psk_table i) in !l
+
+let leak (i:pskid{registered_psk i}) =
+  let (v, _, l) = Somve.v (MM.sel psk_table i) in
+  l := true; v
+
+// Generates a fresh PSK identity
+let fresh_psk_id () : St i:pskid{~ registered_psk i} =
+  let rec subgen () =
+     let id = CoreCrypto.random 8 in
+     match MM.sel psk_table id with
+     | None -> id
+     | Some _ -> subgen () in
+   subgen ()
+
+// "Application PSK" generator (enforces empty session context)
+// Usual caveat of random producing pairwise distinct keys (TODO)
+let gen_psk i:pskid{~ registered_psk i} ctx:psk_context{is_None ctx.session_context} : psk i =
+  let psk = CoreCrypto.random 32 in
+  let leaked = ralloc tls_tables_region false in
+  let add : psk i = (psk, ctx, leaked) in
+  assume (forall j.{:pattern MM.sel psk_table j}
+                   match MM.sel psk_table j with | None -> True
+                   | Some (p,_,_) -> equalBytes p psk <==> equalBytes i j); // TODO
+  MM.extend psk_table i add;
+  add
+
+// Lifted psk_injective lemma
+let registered_psk_injective #i1:pskid #i2:pskid ((p1, _, _):psk i1) ((p2, _, _):psk i2)
+  : Lemma (requires (registered_psk i1) /\ (registered_psk i2))
+    (ensures (equalBytes p1 p2) <==> (equalBytes i1 i2))
+  = admit ()
+
+// Agile "0" hash
+private let zH h =
+  let hL = CoreCrypto.hashSize h in
+  let zeroes = Platform.Bytes.abytes (String.make hL (Char.char_of_int 0)) in
+  CoreCrypto.hash h zeroes
+
+// Resumption context from PSK
+let pskid_rc i:pskid{registered_psk i} =
+  let c = get_psk_context i in
+  match c.resumption_context with
+  | Some b -> CoreCrypto.hash (c.early_hash) b
+  | None -> zH h
+
+// miTLS 0.9:
+// ==========
 // PRF (type pms) -> TLSInfo (type id) -> KEF (extract pms)
 //                     \ StatefulLHAE (coerce id) / 
-
-// Morally, we would like the following types to be
-// abstract, but they must be concrete in order for the definition
-// of id to appear in StatefulLHAE.
-
-//abstract type ms = b:bytes{length b == 48}
+// TODO rework old 1.2 types
 type ms = bytes
 type pms = bytes 
 
-// type pms =
-// | DH_PMS of CommonDH.dhpms // concrete
-// | RSA_PMS of RSAKey.rsapms // concrete
+// Early secrets are indexed by registered PSK identifiers
+type esId = i:pskid{registered_psk i}
+abstract type es (i:esId) =
+  b:bytes{let c = get_psk_context i in length b = CoreCrypto.hashSize c.early_hash}
 
-// Index type for keys; it is morally abstract in
-// StatefulLHAE (but has functions safeId: id->bool,
-// algId: id -> aeAlg) and its concrete definition may
-// be used to prove that StatefulLHAE.gen is not called
-// twice with the same id
-//type id = TLSInfo.id
+// Index of handshake secret
+// Split between DHE, PSK_DHE, and pure PSK
+type hsId =
+  | HSID_PSK: i:esId -> hsId
+  | HSID_PSK_DHE: i:esId -> initiator:CommonDH.share -> responder:CommonDH.share -> hsId
+  | HSID_DHE: h:hashAlg -> initiator:CommonDH.share -> responder:CommonDH.share -> hsId
 
-// (in TLSInfo.fst)
+let hsId_hash = function
+  | HSID_PSK i | HSID_PSK_DHE i _ _ -> let c = get_psk_context i in c.early_hash
+  | HSID_DHE h _ _ -> h
+
+// Get the hashed resumption context
+let hsId_rc = function
+  | HSID_DHE h _ _ -> zH h
+  | HSID_PSK i | HSID_PSK_DHE i _ _ -> pskid_rc i
+
+abstract type hs (i:hsId) =
+  b:bytes{length b = CoreCrypto.hashSize (hsId_hash i)}
+
+// Can be extended with e.g. MSID_staticDH hsid share
+type msId13 =
+  | MSID: hsId:hsId -> msId13
+
+let msId_rc = function
+  | MSID hsId -> hsId_rc hsId
+
+let msId_hash = function
+  | MSID hsId -> hsId_hash hsId
+
+// TLS 1.3 master secret (abstract)
+abstract type ms13 (i:msId13) =
+  b:bytes{length b = CoreCrpyot.hashSize (msId_hash i)}
+
+// Sum of the 3 secret index types
+type secretId =
+  | EarlySecret: i:aeId -> secretId
+  | HandshakeSecret: i:hsId -> secretId
+  | MasterSecret: i:msId13 -> secretId
+
+let secretId_hash = function
+  | EarlySecret i -> esId_hash i
+  | HandshakeSecret i -> hsId_hash i
+  | MasterSecret i -> msId_hash i
+
+// Index of derived secrets
+type derivedID = {
+  underlying_secret: secretId;
+  handshake_log: list HandshakeMessage.hs_msg;
+  label: string;
+}
+
+// RMS index
+type rmsId = i:derivedId {
+  is_MasterSecret i.underlying_secret
+  /\ i.label = "resumption master secret"}
+
+abstract type rms (i:rmsId) =
+  b:bytes{length b = CoreCrpyot.hashSize (secretId_hash i.underlying_secret)}
+
+// Exporter Master Secret (public)
+type exportId = i:derivedId {
+  is_MasterSecret i.underlying_secret
+  /\ i.label = "exporter master secret"}
+
+type exportMS (i:exportId) =
+  b:bytes{length b = CoreCrpyot.hashSize (secretId_hash i.underlying_secret)}
+
+// Index of 1.3 record keys
+type keyId13 = {
+  derived_secret: derivedId;
+  aeadAlg: aeadAlg; // => keySize, ivSize
+  label: string;
+  writer: role;
+}
+
+// Index of Finished keys
+type macId13 = {
+  derived_secret: derivedId;
+  role: role;
+}
+
+// TODO this is superseeded by StAE.state i
+// but I'm waiting for it to be tester to switch over
+// TODO use the newer index types
+type recordInstance =
+| StAEInstance: #id:StreamAE.id -> StreamAE.reader id -> StreamAE.writer id -> recordInstance
+| StLHAEInstance: #id:StatefulLHAE.id -> StatefulLHAE.reader id -> StatefulLHAE.writer id -> recordInstance
+
+// Placeholder until new indexes are propagated outside KS
+let badid ae h writer : TLSInfo.id = {
+    msId = msId;
+    kdfAlg = PRF_SSL3_nested;
+    pv = TLS_1p3;
+    aeAlg = (AEAD ae h);
+    csrConn = bytes_of_hex "";
+    ext = {
+      ne_extended_ms = false;
+      ne_extended_padding = false;
+      ne_secure_renegotiation = RI_Unsupported;
+      ne_supported_groups = None;
+      ne_supported_point_formats = None;
+      ne_server_names = None;
+      ne_signature_algorithms = None;
+      ne_keyShare = None
+    };
+    writer = writer
+  }
+
+// Note from old miTLS (in TLSInfo.fst)
 // type id = {
 //  msId   : msId;            // the index of the master secret used for key derivation
 //  kdfAlg : kdfAlg_t;          // the KDF algorithm used for key derivation
@@ -72,25 +257,22 @@ type pms = bytes
 
 //type exporter_secret = b:bytes{}
 
-// abstract type pre_share_key = b:bytes{}
-//type pre_shared_key = PSK.psk
-
-
 // Agility parameters, extend as needed
 // may be moved to TLSInfo for joint idealization with Handshake
 type ks_alpha12 = pv:protocolVersion * cs:cipherSuite * ems:bool
 type ks_alpha13 = ae:aeadAlg * h:CoreCrypto.hash_alg
 
-// Internal KS state, now with ad-hoc parameters
 type ks_client_state =
 | C_Init: cr:random -> ks_client_state
 | C_12_Resume_CH: cr:random -> si:sessionInfo -> msId:TLSInfo.msId -> ms:ms -> ks_client_state
 | C_12_Full_CH: cr:random -> ks_client_state
 | C_12_wait_MS: csr:csRands -> alpha:ks_alpha12 -> id:TLSInfo.pmsId -> pms:pms -> ks_client_state
 | C_12_has_MS: csr:csRands -> alpha:ks_alpha12 -> id:TLSInfo.msId -> ms:ms -> ks_client_state
-| C_13_1RTT_CH: cr:random -> gs:list (namedGroup * CommonDH.key) -> ks_client_state
-| C_13_1RTT_HTK: alpha:ks_alpha13 -> id:TLSInfo.msId -> xES:ms -> ks_client_state
-| C_13_TS: alpha:ks_alpha13 -> cfk:bytes -> atk0:bytes -> ks_client_state
+| C_13_wait_CH: cr:random -> i:pskid{registered_psk i} -> gs:list (namedGroup * CommonDH.key) -> ks_client_state
+| C_13_wait_SH: cr:random -> es:option (| i:esId & es i & cfk:bytes |) -> gs:list (namedGroup * CommonDH.key) -> ks_client_state
+| C_13_wait_SF: alpha:ks_alpha13 -> cfk:bytes -> sfk:bytes -> (| i:hsId & hs:hs i |) -> ks_client_state
+| C_13_wait_CF: alpha:ks_alpha13 -> cfk:bytes -> late_cfk:bytes -> ms_derived:bytes -> (| i:msId13 & ms:ms13 i |) -> ks_client_state
+| C_13_postHS: alpha:ks_alpha13 -> late_cfk:bytes -> i:msId13 -> ats:bytes -> rms:bytes -> ks_client_state
 | C_Done
 
 type ks_server_state =
@@ -98,8 +280,11 @@ type ks_server_state =
 | S_12_wait_CKE_DH: csr:csRands -> alpha:ks_alpha12 -> our_share:CommonDH.key -> ks_server_state
 | S_12_wait_CKE_RSA: csr: csRands -> alpha:ks_alpha12 -> ks_server_state
 | S_12_has_MS: csr:csRands -> alpha:ks_alpha12 -> id:TLSInfo.msId -> ms:ms -> ks_server_state
-| S_13_1RTT_wait_HTK: alpha:ks_alpha13 -> id:TLSInfo.msId -> xES:ms -> ks_server_state
-| S_13_TS: alpha:ks_alpha13 -> cfk:bytes -> atk0:bytes -> ks_server_state
+| S_13_wait_SH: alpha:ks_alpha13 -> es:option (| i:pskid{registered_psk i} & es i|) -> ks_server_state
+| S_13_wait_SF: alpha:ks_alpha13 -> cfk:bytes -> sfk:bytes -> (| i:hsId & hs:hs i |) -> ks_server_state
+| S_13_wait_CF: alpha:ks_alpha13 -> cfk:bytes -> late_cfk:bytes -> ms_derived:bytes -> (| i:msId13 & ms:ms13 i|) -> ks_server_state
+| S_13_postHS: alpha:ks_alpha13 -> late_cfk:bytes -> i:msId13 -> ats:bytes -> rm
+s:bytes -> ks_server_state
 | S_Done
 
 // Reflecting state separation from HS
@@ -107,24 +292,27 @@ type ks_state =
 | C: s:ks_client_state -> ks_state
 | S: s:ks_server_state -> ks_state
 
+// KeySchedule instances
 type ks =
 | KS: #region:rid -> state:rref region ks_state -> ks
 
-type recordInstance =
-| StAEInstance: #id:StreamAE.id -> StreamAE.reader id -> StreamAE.writer id -> recordInstance
-| StLHAEInstance: #id:StatefulLHAE.id -> StatefulLHAE.reader id -> StatefulLHAE.writer id -> recordInstance
-
-// TODO replace constants (16, 12) with aeadAlg-derived values
-private let expand_13 (h:CoreCrypto.hash_alg) (secret:bytes) (phase:string) (context:bytes) =
-  let cekb = HSCrypto.hkdf_expand_label h
-             secret (phase ^ ", client write key") context 16 in
-  let civb = HSCrypto.hkdf_expand_label h
-             secret (phase ^ ", client write iv") context 12 in
-  let sekb = HSCrypto.hkdf_expand_label h
-             secret (phase ^ ", server write key") context 16 in
-  let sivb = HSCrypto.hkdf_expand_label h
-             secret (phase ^ ", server write iv") context 12 in
+// Extract keys and IVs from a derived 1.3 secret
+private let keygen_13 h secret phase ae =
+  let kS = CoreCrypto.aeadKeySize ae in
+  let iS = CoreCrypto.aeadRealIVSize ae in
+  let f x y = HSCrypto.hkdf_expand_label h secret (phase ^ x) empty_bytes y in
+  let cekb = f ", client write key" kS in
+  let civb = f ", client write iv" iS in
+  let sekb = f ", server write key" kS in
+  let sivb = f ", server write iv" iS in
   (cekb,civb,sekb,sivb)
+
+// Extract finished keys
+private let finished_13 h secret =
+  let hL = CoreCrypto.hashSize h in
+  let cfk = HSCrypto.hkdf_expand_label h ms "client finished" empty_bytes hL in
+  let sfk = HSCrypto.hkdf_expand_label h ms "server finished" empty_bytes hL in
+  cfk, sfk
 
 val ks_client_random: ks:ks -> ST random
   (requires fun h0 ->
@@ -164,7 +352,7 @@ let create #rid r =
     | Server -> S (S_Init nonce) in
   (KS #ks_region (ralloc ks_region istate)), nonce
 
-val ks_client_13_init_1rtt: ks:ks -> list (g:namedGroup{is_SEC g \/ is_FFDHE g}) -> ST (list (namedGroup * bytes))
+val ks_client_13_1rtt_init: ks:ks -> list (g:namedGroup{is_SEC g \/ is_FFDHE g}) -> ST (list (namedGroup * bytes))
   (requires fun h0 ->
     let kss = sel h0 (KS.state ks) in
     is_C kss /\ is_C_Init (C.s kss))
@@ -173,16 +361,95 @@ val ks_client_13_init_1rtt: ks:ks -> list (g:namedGroup{is_SEC g \/ is_FFDHE g})
     modifies (Set.singleton rid) h0 h1
     /\ modifies_rref rid !{as_ref st} h0 h1)
 
-let ks_client_13_init_1rtt ks groups =
+let ks_client_13_1rtt_init ks groups =
   let KS #rid st = ks in
   let C (C_Init cr) = !st in
   let kg x = x, (match x with
     | SEC ecg -> CommonDH.keygen (CommonDH.ECDH ecg)
     | FFDHE g -> CommonDH.keygen (CommonDH.FFDH (DHGroup.Named g))) in
   let gs = List.Tot.map kg groups in
-  st := C (C_13_1RTT_CH cr gs);
+  st := C (C_13_wait_SH cr None gs);
   let pub (x,y) = x, CommonDH.serialize_raw y in
   List.Tot.map pub gs
+
+val ks_client_13_0rtt_init: ks:ks -> i:pskid{registered_psk i} -> list (g:namedGroup{is_SEC g \/ is_FFDHE g}) -> ST (list (namedGroup * bytes))
+  (requires fun h0 ->
+    let kss = sel h0 (KS.state ks) in
+    is_C kss /\ is_C_Init (C.s kss))
+  (ensures fun h0 r h1 ->
+    let KS #rid st = ks in
+    modifies (Set.singleton rid) h0 h1
+    /\ modifies_rref rid !{as_ref st} h0 h1)
+
+let ks_client_13_0rtt_init ks pskid groups =
+  let KS #rid st = ks in
+  let C (C_Init cr) = !st in
+  let kg x = x, (match x with
+    | SEC ecg -> CommonDH.keygen (CommonDH.ECDH ecg)
+    | FFDHE g -> CommonDH.keygen (CommonDH.FFDH (DHGroup.Named g))) in
+  let gs = List.Tot.map kg groups in
+  st := C (C_13_wait_CH cr pskid gs);
+  let pub (x,y) = x, CommonDH.serialize_raw y in
+  List.Tot.map pub gs
+
+// Derive the early keys from the early secret
+let ks_client_13_0rtt_ch ks log_hash
+  : ST (recordInstance * recordInstance)
+  (requires fun h0 ->
+    let kss = sel h0 (KS.state ks) in
+    is_C kss /\ is_C_Init (C.s kss))
+  (ensures fun h0 r h1 ->
+    let KS #rid st = ks in
+    modifies (Set.singleton rid) h0 h1
+    /\ modifies_rref rid !{as_ref st} h0 h1) =
+  let KS #rid st = ks in
+  let C (C_13_wait_CH cr pskid gs) = !st in
+  let (psk, ctx, _) = Some.v (MM.sel psk_table pskid) in
+  let h, ae = c.early_hash, c.early_ae in
+  let hL = CoreCrypto.hashSize h in
+  let zeroes = Platform.Bytes.abytes (String.make hL (Char.char_of_int 0)) in
+  let es : es pskid = HSCrypto.hkdf_extract h zeroes psk in
+  let sh_rctx = log_hash @| (pskid_rc pskid) in
+  let es_derived = HSCrypto.hkdf_expand_label h hs "early traffic secret" sh_rctx hL in
+
+  // Expand all keys from the derived early secret
+  let (ck,civ, _, _) = keygen_13 h es_derived "early traffic key expansion" ae in
+  let (ck',civ', _, _) = keygen_13 h es_derived "early application data key expansion" ae in
+  let (cfk, _) = finished_13 h es_derived in
+
+  let id = badid ae h Client in
+  let ckv: StreamAE.key id = ck in
+  let civ: StreamAE.iv id  = civ in
+  let rw = StreamAE.coerce HyperHeap.root id ckv civ in
+  let r = StreamAE.genReader HyperHeap.root rw in
+  let early_hs = StAEInstance r w
+
+  let id = badid ae h Client in
+  let ckv: StreamAE.key id = ck' in
+  let civ: StreamAE.iv id  = civ' in
+  let rw = StreamAE.coerce HyperHeap.root id ckv civ in
+  let r = StreamAE.genReader HyperHeap.root rw in
+  let early_d = StAEInstance r w
+
+  let (ck,civ, _, _) = keygen_13 h es_derived "early application data key expansion" ae in
+  let (cfk, _) = finished_13 h es_derived in
+ 
+  st := C (C_13_wait_SH cr (Some (pskid, es, cfk)) gs);
+  (early_hs, early_d)
+
+val ks_client_13_0rtt_finished: ks:ks -> log_hash:bytes -> ST (cvd:bytes)
+  (requires fun h0 ->
+    let kss = sel h0 (KS.state ks) in
+    is_C kss /\ is_C_13_wait_SH (C.s kss))
+  (ensures fun h0 r h1 -> h0 = h1)
+
+// Compute 0-RTT finished
+let ks_client_13_0rtt_finished ks log_hash =
+  let KS #rid st = ks in
+  let C (C_13_wait_SH cr (Some (pskid, es, cfk)) gs) = !st in
+  let (psk, ctx, _) = Some.v (MM.sel psk_table pskid) in
+  let h = c.early_hash in
+  CoreCrypto.hmac h cfk (log_hash |@ (pskid_rc pskid))
 
 // Called before sending client hello
 // (the external style of resumption may become internal to protect ms abstraction)
@@ -233,7 +500,29 @@ let ks_server_12_init_dh ks cr pv cs ems group =
   st := S (S_12_wait_CKE_DH csr (pv, cs, ems) our_share);
   our_share
 
-val ks_server_13_1rtt_init: ks:ks -> cr:random -> cs:cipherSuite -> gn:namedGroup -> gxb:bytes -> ST bytes
+private let s13_dh gn gxb =
+  let gx = match gn with
+    | SEC ec ->
+      let Some gx = CommonDH.parse (CommonDH.ECP (ECGroup.params_of_group ec)) gxb in gx
+    | FFDHE ff ->
+      let Some gx =  CommonDH.parse (CommonDH.FFP (DHGroup.params_of_group (DHGroup.Named ff))) gxb in gxi
+  in let gy, gxy = CommonDH.dh_responder gx in
+  (gy, 
+
+val ks_server_13_0rtt_init: ks:ks -> cr:random -> i:pskid{registered_psk i} -> cs:cipherSuite -> gn:namedGroup -> gxb:bytes -> log_hash:bytes -> ST (recordInstance * recordInstance * our_share:bytes)
+  (requires fun h0 ->
+    let kss = sel h0 (KS.state ks) in
+    is_S kss /\ is_S_Init (S.s kss)
+    /\ is_CipherSuite cs /\ (let CipherSuite kex _ _ = cs in
+       (kex = Kex_PSK_DHE \/ kex = Kex_PSK_ECDHE)))
+  (ensures fun h0 r h1 ->
+    let KS #rid st = ks in
+    modifies (Set.singleton rid) h0 h1
+    /\ modifies_rref rid !{as_ref st} h0 h1)
+
+// let ks_server13_0rtt_init ks cr pskid cs gn gxb log_hash = () // TODO
+
+val ks_server_13_1rtt_init: ks:ks -> cr:random -> cs:cipherSuite -> gn:namedGroup -> gxb:bytes -> ST (our_share:bytes)
   (requires fun h0 ->
     let kss = sel h0 (KS.state ks) in
     is_S kss /\ is_S_Init (S.s kss)
@@ -248,49 +537,49 @@ val ks_server_13_1rtt_init: ks:ks -> cr:random -> cs:cipherSuite -> gn:namedGrou
 let ks_server_13_1rtt_init ks cr cs gn gxb =
   let KS #region st = ks in
   let S (S_Init sr) = !st in
-  let gx = match gn with
-    | SEC ec ->
-      let Some gx = CommonDH.parse (CommonDH.ECP (ECGroup.params_of_group ec)) gxb in gx
-    | FFDHE ff ->
-      let Some gx =  CommonDH.parse (CommonDH.FFP (DHGroup.params_of_group (DHGroup.Named ff))) gxb in gx in
   let CipherSuite _ _ (AEAD ae h) = cs in
-  let our_share, gxy = CommonDH.dh_responder gx in
-  let zeroes = Platform.Bytes.abytes (String.make 32 (Char.char_of_int 0)) in
-  let msId = noMsId in
-  let xES = HSCrypto.hkdf_extract h zeroes gxy in
-  st := S (S_13_1RTT_wait_HTK (ae, h) msId xES);
+  let our_share, gxy = s13_dh gn gxb in
+  let hsId = HSID h 
+  let hs = HSCrypto.hkdf_extract h zeroes gxy in
+  st := S (S_13_wait_SH (ae, h) msId xES);
   CommonDH.serialize_raw our_share
 
-val ks_server_13_get_htk: ks:ks -> log_hash:bytes -> ST recordInstance
+val ks_server_13_sh: ks:ks -> log_hash:bytes -> ST recordInstance
   (requires fun h0 ->
     let kss = sel h0 (KS.state ks) in
-    is_S kss /\ is_S_13_1RTT_wait_HTK (S.s kss))
-  (ensures fun h0 r h1 -> h0 = h1)
+    is_S kss /\ is_S_13_wait_SH (S.s kss))
+  (ensures fun h0 r h1 ->
+    let KS #rid st = ks in
+    modifies (Set.singleton rid) h0 h1
+    /\ modifies_rref rid !{as_ref st} h0 h1)
 
 let ks_server_13_get_htk ks log_hash =
   let KS #region st = ks in
-  let S (S_13_1RTT_wait_HTK (ae, h) msId xES) = !st in
+  let S (S_13_wait_SH (ae, h) es gxy) = !st in
+  let hL = CoreCrypto.hashSize h in
+  let zeroes = Platform.Bytes.abytes (String.make hL (Char.char_of_int 0)) in
+
+  // Early secret: must derive zero here as hash is not known before
+  let es, rctx =
+    match es with
+    // Application-PSK may have an empty resumption contexct
+    | Some (i, es) ->
+      let ctx = get_psk_context i in
+      es, (match ctx.resumption_context with
+      | None -> zeroes | Some rc -> rc)
+    | None -> HSCrypto.hkdf_extract h zeroes zeroes, zH h
+  in
+
+  // Handshake secret
+  let is = CommonDH.share_of_key gx in
+  let rs = CommonDH.share_of_key gy in
+  let hsId = match es with
+    | None -> HSID h is rs
+    | Some (pskid, _) -> HSID_PSK_DHE pskid is rs in
+
+  let hs : hs hsId = HSCrypto.hkdf_extract h es gxy in
   let (ck,civ,sk,siv) = expand_13 h xES "handshake key expansion" log_hash in
-  // TODO fix the broken index of StreamAE
-  let id = {
-    msId = msId;
-    kdfAlg = PRF_SSL3_nested;
-    pv = TLS_1p3;
-    aeAlg = (AEAD ae h);
-    csrConn = bytes_of_hex "";
-    ext = {
-      ne_extended_ms = false;
-      ne_extended_padding = false;
-      ne_secure_renegotiation = RI_Unsupported;
-      ne_supported_groups = None;
-      ne_supported_point_formats = None;
-      ne_server_names = None;
-      ne_signature_algorithms = None;
-      ne_keyShare = None
-    };
-    writer = Server
-  } in
-  assume (~ (authId id));
+  let id = badid ae h Server in
   let ckv: StreamAE.key id = ck in
   let civ: StreamAE.iv id  = civ in
   let skv: StreamAE.key id = sk in
@@ -298,6 +587,7 @@ let ks_server_13_get_htk ks log_hash =
   let w = StreamAE.coerce HyperHeap.root id skv siv in
   let rw = StreamAE.coerce HyperHeap.root id ckv civ in
   let r = StreamAE.genReader HyperHeap.root rw in
+  st := S (S_13_wait_SF (ae, h) cfk sfk (hsId, hs));
   StAEInstance r w
 
 // log is the raw HS log, used for EMS derivation
@@ -356,45 +646,53 @@ let ks_client_12_resume ks sr pv cs =
 //   2. they use different return types
 //   3. they are called at different locations
 
-val ks_client_13_1rtt: ks:ks -> cs:cipherSuite -> gy:(namedGroup * bytes) -> log_hash:bytes -> ST recordInstance
+val ks_client_13_sh: ks:ks -> cs:cipherSuite -> gy:(namedGroup * bytes) -> accept_early_data:bool -> log_hash:bytes -> ST recordInstance
   (requires fun h0 ->
     let kss = sel h0 (KS.state ks) in
-    is_C kss /\ is_C_13_1RTT_CH (C.s kss))
+    is_C kss /\ is_C_13_wait_SH (C.s kss) /\ 
+    // Ensure consistency of ae/h if 0-RTT data is accepted
+    (let C_13_wait_SH _ ei _ = C.s kss in
+     match ei with | None -> True | Some id, _, _ ->
+       let CipherSuite _ _ (AEAD ae h) = cs in
+       let ctxt = get_psk_context id in
+       accept_early_data ==> ctxt.early_ae = ae /\ ctxt.early_hash = h))
   (ensures fun h0 r h1 ->
     let KS #rid st = ks in
     modifies (Set.singleton rid) h0 h1
     /\ modifies_rref rid !{as_ref st} h0 h1)
 
-let ks_client_13_1rtt ks cs (gs, gyb) log_hash =
+// ServerHello log breakpoint (client)
+let ks_client_13_sh ks cs (gs, gyb) accept_ed log_hash =
   let KS #region st = ks in
-  let C (C_13_1RTT_CH cr gc) = !st in
-  let Some (_, gx) = List.Tot.find (fun (gc,_) -> gc=gs) gc in
+  let C (C_13_wait_SH cr early_info gc) = !st in
+  let Some (_, gx) = List.Tot.find (fun (gc,_) -> gc = gs) gc in
   let Some gy = CommonDH.parse (CommonDH.key_params gx) gyb in
   let gxy = CommonDH.dh_initiator gx gy in
   let CipherSuite _ _ (AEAD ae h) = cs in
-  let zeroes = Platform.Bytes.abytes (String.make 32 (Char.char_of_int 0)) in
-  let msId = noMsId in
-  let xES = HSCrypto.hkdf_extract h zeroes gxy in
-  let (ck,civ,sk,siv) = expand_13 h xES "handshake key expansion" log_hash in
-  // TODO fix the broken index of StreamAE
-  let id = {
-    msId = msId;
-    kdfAlg = PRF_SSL3_nested;
-    pv = TLS_1p3;
-    aeAlg = (AEAD ae h);
-    csrConn = bytes_of_hex "";
-    ext = {
-      ne_extended_ms = false;
-      ne_extended_padding = false;
-      ne_secure_renegotiation = RI_Unsupported;
-      ne_supported_groups = None;
-      ne_supported_point_formats = None;
-      ne_server_names = None;
-      ne_signature_algorithms = None;
-      ne_keyShare = None
-    };
-    writer = Client
-  } in
+  let hL = CoreCrypto.hashSize h in
+  let zeroes = Platform.Bytes.abytes (String.make hL (Char.char_of_int 0)) in
+
+  // Early secret: must derive zero here as hash is not known before
+  let es =
+    match early_info, accept_ed with
+    | Some (_, es, _), true -> es
+    | _ -> HSCrypto.hkdf_extract h zeroes zeroes in
+
+  // Handshake secret
+  let is = CommonDH.share_of_key gx in
+  let rs = CommonDH.share_of_key gy in
+  let hsId = match early_info with
+    | None -> HSID h is rs
+    | Some (pskid, _, _) -> HSID_PSK_DHE pskid is rs in
+  let hs : hs hsId = HSCrypto.hkdf_extract h es gxy in
+
+  // Derived handshake secret
+  let sh_rctx = log_hash @| (hsId_rc hsId) in
+  let hs_derived = HSCrypto.hkdf_expand_label h hs "handshake traffic secret" sh_rctx hL in
+  let (ck,civ,sk,siv) = keygen_13 h hs_derived "handshake key expansion" ae in
+  let (cfk, sfk) = finished_13 h hs_derived in
+
+  let id = badid ae h Client in
   assume (~ (authId id));
   let ckv: StreamAE.key id = ck in
   let civ: StreamAE.iv id  = civ in
@@ -403,34 +701,33 @@ let ks_client_13_1rtt ks cs (gs, gyb) log_hash =
   let siv: StreamAE.iv id  = siv in
   let rw = StreamAE.coerce HyperHeap.root id skv siv in
   let r = StreamAE.genReader HyperHeap.root rw in
-  st := C (C_13_1RTT_HTK (ae, h) msId xES);
+  st := C (C_13_wait_SF (ae, h) cfk sfk (hsId, hs));
   StAEInstance r w
 
 // Old KS: ms, cfk, sfk is up to CertificateVerify
 // application keys use atk with context up to server finished
-val ks_client_13_1rtt_server_finished: ks:ks -> log_hash:bytes -> ST (svd:bytes)
+val ks_client_13_server_finished: ks:ks -> log_hash:bytes -> ST (svd:bytes)
   (requires fun h0 ->
     let kss = sel h0 (KS.state ks) in
-    is_C kss /\ is_C_13_1RTT_HTK (C.s kss))
-  (ensures fun h0 r h1 ->
-    let KS #rid st = ks in
-    modifies (Set.singleton rid) h0 h1
-    /\ modifies_rref rid !{as_ref st} h0 h1)
+    is_C kss /\ is_C_13_wait_SF (C.s kss))
+  (ensures fun h0 r h1 -> h0 = h1)
 
-let ks_client_13_1rtt_server_finished ks log_hash =
+let ks_client_13_server_finished ks log_hash =
   let KS #region st = ks in
-  let C (C_13_1RTT_HTK alpha msId xES) = !st in
+  let C (C_13_wait_SF alpha cfk sfk (hsId, hs)) = !st in
   let (ae, h) = alpha in
-  let mSS = HSCrypto.hkdf_expand_label h xES "expanded static secret" log_hash 32 in
-  let mES = HSCrypto.hkdf_expand_label h xES "expanded ephemeral secret" log_hash 32 in
-  let ms = HSCrypto.hkdf_extract h mSS mES in
+  CoreCrypto.hmac h sfk (log_hash @| (hsId_rc hsId))
 
-  let cfk = HSCrypto.hkdf_expand_label h ms "client finished" empty_bytes 32 in
-  let sfk = HSCrypto.hkdf_expand_label h ms "server finished" empty_bytes 32 in
-  let ts0 = HSCrypto.hkdf_expand_label h ms "traffic secret" log_hash 32 in
-  let svd = CoreCrypto.hmac h sfk log_hash in
-  st := C (C_13_TS alpha cfk ts0);
-  svd
+val ks_client_13_client_finished: ks:ks -> log_hash:bytes -> ST (cvd:bytes)
+  (requires fun h0 ->
+    let kss = sel h0 (KS.state ks) in
+    is_C kss /\ is_C_13_wait_CF (C.s kss))
+  (ensures fun h0 r h1 -> h0 = h1)
+
+let ks_client_13_client_finished ks log_hash =
+  let KS #region st = ks in
+  let C (C_13_wait_CF (_, h) cfk _ _ (msId, _)) = !st in
+  CoreCrypto.hmac h cfk (log_hash @| (msId_rc msId))
 
 val ks_server_13_server_finished: ks:ks -> log_hash:bytes -> ST (svd:bytes)
   (requires fun h0 ->
@@ -499,40 +796,31 @@ let ks_server_13_client_finished ks log_hash =
   st := S (S_Done);
   (cvd, StAEInstance r w)
 
-val ks_client_13_1rtt_client_finished: ks:ks -> log_hash:bytes -> ST (cvd:bytes * recordInstance)
+val ks_client_13_sf: ks:ks -> log_hash:bytes -> ST (recordInstance)
   (requires fun h0 ->
     let kss = sel h0 (KS.state ks) in
-    is_C kss /\ is_C_13_TS (C.s kss))
+    is_C kss /\ is_C_13_wait_SF (C.s kss))
   (ensures fun h0 r h1 ->
     let KS #rid st = ks in
     modifies (Set.singleton rid) h0 h1
     /\ modifies_rref rid !{as_ref st} h0 h1)
 
-let ks_client_13_1rtt_client_finished ks log_hash =
+let ks_client_13_sf ks log_hash =
   let KS #region st = ks in
-  let C (C_13_TS alpha cfk ts0) = !st in
+  let C (C_13_wait_SF alpha cfk _ (hsId, hs)) = !st in
   let (ae, h) = alpha in
-  let cvd = CoreCrypto.hmac h cfk log_hash in
-  let (ck,civ,sk,siv) = expand_13 h ts0 "application data key expansion" log_hash in
-  // TODO need to completely scrap and redo 1.3 index types
-  let id = {
-    msId = noMsId;
-    kdfAlg = PRF_SSL3_nested;
-    pv = TLS_1p3;
-    aeAlg = (AEAD ae h);
-    csrConn = bytes_of_hex "";
-    ext = {
-      ne_extended_ms = false;
-      ne_extended_padding = false;
-      ne_secure_renegotiation = RI_Unsupported;
-      ne_supported_groups = None;
-      ne_supported_point_formats = None;
-      ne_server_names = None;
-      ne_signature_algorithms = None;
-      ne_keyShare = None
-    };
-    writer = Client
-  } in
+  let hL = CoreCrypto.hashSize h in
+  let zeroes = Platform.Bytes.abytes (String.make hL (Char.char_of_int 0)) in
+
+  let msId = MSID hsId in
+  let ms : ms13 msId = HSCrypto.hkdf_extract h hs zeroes in
+
+  let sh_rctx = log_hash @| (hsID_rc hsId) in
+  let ms_derived = HSCrypto.hkdf_expand_label h ms "application traffic secret" sh_rctx hL in
+  let (ck,civ,sk,siv) = keygen_13 h ms_derived "application data key expansion" in
+  let (late_cfk, _) = finished_13 h ms_derived in
+
+  let id = badid ae h Client in
   let ckv: StreamAE.key id = ck in
   let civ: StreamAE.iv id  = civ in
   let w = StreamAE.coerce HyperHeap.root id ckv civ in
@@ -540,8 +828,29 @@ let ks_client_13_1rtt_client_finished ks log_hash =
   let siv: StreamAE.iv id  = siv in
   let rw = StreamAE.coerce HyperHeap.root id skv siv in
   let r = StreamAE.genReader HyperHeap.root rw in
-  st := C (C_Done);
-  (cvd, StAEInstance r w)
+  st := C (C_13_wait_CF alpha cfk late_cfk ms_derived (msId, ms));
+  StAEInstance r w
+
+val ks_client_13_cf: ks:ks -> log_hash:bytes -> ST (| i:msId & exportMS i |)
+  (requires fun h0 ->
+    let kss = sel h0 (KS.state ks) in
+    is_C kss /\ is_C_13_wait_CF (C.s kss))
+  (ensures fun h0 r h1 ->
+    let KS #rid st = ks in
+    modifies (Set.singleton rid) h0 h1
+    /\ modifies_rref rid !{as_ref st} h0 h1)
+
+let ks_client_13_cf ks log_hash =
+  let KS #region st = ks in
+  let C (C_13_wait_CF alpha cfk late_cfk ms_derived (msId, ms)) = !st in
+  let (ae, h) = alpha in
+  let hL = CoreCrypto.hashSize h in
+  let sh_rctx = log_hash @| (msID_rc msId) in
+  let rms = HSCrypto.hkdf_expand_label h ms "resumption master secret" sh_rctx hL in
+  let ems : exportMS msId = HSCrypto.hkdf_expand_label h ms "resumption master secret" sh_rctx hL in
+  let ts = HSCrypto.hkdf_expand_label h ms_derived "traffic secret" sh_rctx hL in
+  st := C (C_13_postHS alpha late_cfk msId ts rms);
+  (msId, ems)
 
 // Called by Hanshake when DH key echange is negotiated
 val ks_client_12_full_dh: ks:ks -> sr:random -> pv:protocolVersion -> cs:cipherSuite -> ems:bool -> peer_share:CommonDH.key -> ST CommonDH.key
